theories/LambdaANF/LambdaBox_to_LambdaANF_common.v
@@ -1,0 +1,181 @@
+(* Common definitions for converting MetaRocq Erasure (EAst.term) to LambdaANF *)
+
+From Stdlib Require Import ZArith.ZArith Lists.List Arith.Arith.
+From CertiRocq Require Import Common.AstCommon Common.compM Pipeline_utils.
+
+From MetaRocq.Erasure Require Import EAst.
+From MetaRocq.Utils Require Import bytestring.
+
+Require Import LambdaANF.cps LambdaANF.ctx LambdaANF.state.
+Require Import compcert.lib.Maps.
+
+Require Import ExtLib.Structures.Monads.
+
+Import ListNotations.
+Import Monad.MonadNotation.
+Open Scope monad_scope.
+Open Scope bs_scope.
+
+Local Notation string := bytestring.string.
+
+(** * Constructor discriminant *)
+
+Definition dcon : Set := inductive * N.
+
+Definition dcon_of_con (i : inductive) (n : nat) : dcon := (i, N.of_nat n).
+
+(** * Constructor tag mapping *)
+
+Definition conId_map := list (dcon * ctor_tag).
+
+Theorem conId_dec: forall x y:dcon, {x = y} + {x <> y}.
+Proof.
+  intros. destruct x,y.
+  assert (H:= AstCommon.inductive_dec i i0).
+  destruct H.
+  - destruct (classes.eq_dec n n0).
+    + subst. left. auto.
+    + right. intro. apply n1. inversion H. auto.
+  - right; intro; apply n1. inversion H; auto.
+Defined.
+
+Section TagLookup.
+
+  Context (default_tag : positive).
+
+  Fixpoint dcon_to_info (a:dcon) (sig:conId_map) :=
+    match sig with
+    | nil => default_tag
+    | ((cId, inf)::sig') => match conId_dec a cId with
+                            | left _ => inf
+                            | right _ => dcon_to_info a sig'
+                            end
+    end.
+
+  Definition dcon_to_tag (a:dcon) (sig:conId_map) :=
+    dcon_to_info a sig.
+
+End TagLookup.
+
+Definition constr_env : Type := conId_map.
+
+(** * Global constant environment *)
+
+(** Map from global constant names to LambdaANF variables.
+    Built when processing the global environment; used to translate [tConst]. *)
+Definition const_map := list (kername * var).
+
+Fixpoint lookup_const (cm : const_map) (k : kername) : option var :=
+  match cm with
+  | [] => None
+  | (k', v) :: cm' =>
+    if eq_kername k k' then Some v else lookup_const cm' k
+  end.
+
+(** Primitive lookup *)
+Fixpoint find_prim (prims : list (primitive * positive)) (n : kername) : option positive :=
+  match prims with
+  | [] => None
+  | (prim, pos) :: prims =>
+    if eq_kername n prim.(prim_name) then Some pos else find_prim prims n
+  end.
+
+
+(** * Inductive environment processing *)
+
+Definition ienv := list (Kernames.kername * AstCommon.itypPack).
+
+Fixpoint fromN (n:positive) (m:nat) : list positive * positive :=
+  match m with
+  | O => (nil, n)
+  | S m' =>
+    let (l, nm) := (fromN (n+1) (m')) in
+    (n::l, nm)
+  end.
+
+(** Bind m projections. The first variable in the list binds the last constructor argument. *)
+Fixpoint ctx_bind_proj (tg:ctor_tag) (r:positive) (vars : list var) (args:nat)
+  : exp_ctx :=
+  match vars with
+  | [] => Hole_c
+  | v :: vars =>
+    let ctx_p' := ctx_bind_proj tg r vars (args - 1) in
+    (Eproj_c v tg (N.of_nat (args - 1)) r ctx_p')
+  end.
+
+Section InductiveEnv.
+
+  Context (default_tag default_itag : positive).
+
+  Fixpoint convert_cnstrs (tyname:string) (cct:list ctor_tag) (itC:list AstCommon.Cnstr)
+           (ind:Kernames.inductive) (nCon:N) (unboxed : N) (boxed : N)
+           (niT:ind_tag) (ce:ctor_env) (dcm:conId_map) :=
+    match (cct, itC) with
+    | (cn::cct', cst::icT') =>
+      let (cname, ccn) := cst in
+      let is_unboxed := Nat.eqb ccn 0 in
+      let info := {| ctor_name := BasicAst.nNamed cname
+                     ; ctor_ind_name := BasicAst.nNamed tyname
+                     ; ctor_ind_tag := niT
+                     ; ctor_arity := N.of_nat ccn
+                     ; ctor_ordinal := if is_unboxed then unboxed else boxed
+                  |} in
+      convert_cnstrs tyname cct' icT' ind (nCon+1)%N
+                     (if is_unboxed then unboxed + 1 else unboxed)
+                     (if is_unboxed then boxed else boxed + 1)
+                     niT
+                     (M.set cn info ce)
+                     (((ind,nCon), cn)::dcm)
+    | (_, _) => (ce, dcm)
+    end.
+
+  Fixpoint convert_typack typ (idBundle:Kernames.kername) (n:nat)
+           (ice : (ind_env * ctor_env * ctor_tag * ind_tag * conId_map))
+    : (ind_env * ctor_env * ctor_tag * ind_tag * conId_map) :=
+    let '(ie, ce, ncT, niT, dcm) := ice in
+    match typ with
+    | nil => ice
+    | (AstCommon.mkItyp itN itC) :: typ' =>
+      let (cct, ncT') := fromN ncT (List.length itC) in
+      let (ce', dcm') :=
+          convert_cnstrs itN cct itC (Kernames.mkInd idBundle n) 0 0 0 niT ce dcm
+      in
+      let ityi :=
+          combine cct (map (fun (c:AstCommon.Cnstr) =>
+                              let (_, n) := c in N.of_nat n) itC)
+      in
+      convert_typack typ' idBundle (n+1)
+                     (M.set niT ityi ie, ce', ncT', (Pos.succ niT), dcm')
+    end.
+
+  Fixpoint convert_env' (g:ienv) (ice:ind_env * ctor_env * ctor_tag * ind_tag * conId_map)
+    : (ind_env * ctor_env * ctor_tag * ind_tag * conId_map) :=
+    let '(ie, ce, ncT, niT, dcm) := ice in
+    match g with
+    | nil => ice
+    | (id, ty)::g' =>
+      convert_env' g' (convert_typack ty id 0 (ie, ce, ncT, niT, dcm))
+    end.
+
+  Definition convert_env (g:ienv): (ind_env * ctor_env * ctor_tag * ind_tag * conId_map) :=
+    let default_ind_env := M.set default_itag (cons (default_tag, 0%N) nil) (M.empty ind_ty_info) in
+    let info := {| ctor_name := BasicAst.nAnon
+                   ; ctor_ind_name := BasicAst.nAnon
+                   ; ctor_ind_tag := default_itag
+                   ; ctor_arity := 0%N
+                   ; ctor_ordinal := 0%N
+                |} in
+    let default_ctor_env := M.set default_tag info (M.empty ctor_ty_info) in
+    convert_env' g (default_ind_env, default_ctor_env, (Pos.succ default_tag:ctor_tag), (Pos.succ default_itag:ind_tag), nil).
+
+End InductiveEnv.
+
+
+(** * Helper: pad name list to given length *)
+
+Fixpoint names_lst_len (ns : list name) (m : nat) : list name :=
+  match ns, m with
+  | _, 0%nat => []
+  | [], S _ => repeat nAnon m
+  | n :: ns, S m => n :: names_lst_len ns m
+  end.
